refactoring

.coqdeps.d
@@ -1,5 +1,7 @@
-ATL.vo ATL.glob ATL.v.beautified: ATL.v
-ATL.vio: ATL.v
+NonEmpty.vo NonEmpty.glob NonEmpty.v.beautified: NonEmpty.v
+NonEmpty.vio: NonEmpty.v
+ATL.vo ATL.glob ATL.v.beautified: ATL.v NonEmpty.vo
+ATL.vio: ATL.v NonEmpty.vio
 VNM.vo VNM.glob VNM.v.beautified: VNM.v ATL.vo
 VNM.vio: VNM.v ATL.vio
 test.vo test.glob test.v.beautified: test.v ATL.vo
