ATL.v
@@ -4,6 +4,8 @@ Require Export Classical.
 Require Export Decidable.
 Require Export FunctionalExtensionality.
 
+
+Require Import NonEmpty.
 Require Import Coq.Lists.List Coq.Bool.Bool.
 
 Import Coq.Lists.List.ListNotations.
@@ -17,9 +19,9 @@ Parameter Move : Set.           (* alphabet of moves individual players can make
 *)
 Parameter beq_state : State -> State -> bool.
 Parameter beq_player : Player -> Player -> bool.
-
+Parameter beq_observable : Observable -> Observable -> bool.
 (* type corresponding to the set of moves each player makes. *)
-Definition move_vec (q: State) := forall (p:Player), Move.
+Definition move_vec := State -> Player -> Move.
 
 (* AHK says not all moves are available at all states. We express this using a function type [enabled], expressing which moves are available at which state.  *)
 Definition enabled := State -> Player -> Move -> bool.
@@ -28,7 +30,7 @@ Definition enabled := State -> Player -> Move -> bool.
 Definition observation := State -> Observable.
 
 (* transition function. *)
-Definition delta := forall (q:State), move_vec q -> State.
+Definition delta := State -> move_vec -> State.
 
 Record CGS : Set := mkRat
                       {
@@ -43,160 +45,151 @@ Record CGS : Set := mkRat
 
 (* property of states [q] and [q'], expressind whether [q'] can be reached from [q] in game [g], under [g]'s transition function.*)
 Definition succ (g:CGS) (q q':State) :=
-  exists mv:move_vec q,
+  exists mv:move_vec,
     (forall (p:Player),
-        (g.(e) q p (mv p)) = true) /\
+        (g.(e) q p (mv q p)) = true) /\
     q'=g.(d) q mv.
 
 (* Computations are nonempty sequences of states [l] where every [l_(i+1)] is a successor of [l_i]. *)
 
-(* [computation_property_fix] checks that successive states are successors according to the above property. *)
-Fixpoint computation_property_fix (g:CGS) (l:list State) : Prop :=
-  match l with
-  | nil => False
-  | x::l' => match hd_error l' with
-             | None => True
-             | Some y => succ g x y /\ computation_property_fix g l'
-             end
-  end.
 
-(* A q-computation starts with state [q]. [computation_property] checks for this, and for [computation_property_fix] to hold.*)
-Definition computation_property (g:CGS) (q:State) (l:list State) : Prop :=
-  (hd_error l) = Some q /\ computation_property_fix g l.
+(* [computation_property_fix] checks that successive states are successors according to the above property. *)
+
+Inductive computation_property: CGS -> State -> nonempty State -> Prop :=
+| computation_property_one: forall (g: CGS) (s: State),
+    computation_property g s (s:::nil)
+| computation_property_cons: forall (g: CGS) (ss: list State) (s1 s2: State)
+    (FIXSUCC: computation_property g s2 (s2 :::ss ))
+    (SUCC: succ g s1 s2),
+    computation_property g s1 (s1:::s2::ss).
+
+
 
 (* Subset type of [list State] where [computation_property] holds. *)
-Definition computation (g:CGS) (q:State) : Set := {l:list State | @computation_property g q l}.
+(* )Definition computation (g:CGS) (q:State) : Set := {l:list State | computation_property g q l}.
+ *)
+
 
 (* If a [list State] is a [q]-computation, that same [list State] cons'ed with State [a] is an [a]-computation. *)
-Theorem computation_property_cons :
-  forall (g:CGS) (l:list State) (q a b:State),
-    computation_property g q (b::l) /\ succ g a b -> computation_property g a (a::b::l).
-Proof.
-  intros. destruct H. destruct H. unfold computation_property. split.
-  - reflexivity.
-  - simpl. split.
-    + apply H0.
-    + simpl in H1. apply H1.
-Qed.
+(* Theorem computation_property_cons : *)
+(*   forall (g:CGS) (l:list State) (q a b:State), *)
+(*     computation_property g q (b::l) /\ succ g a b -> computation_property g a (a::b::l). *)
+(* Proof. *)
+(*   intros. destruct H. destruct H. unfold computation_property. split. *)
+(*   - reflexivity. *)
+(*   - simpl. split. *)
+(*     + apply H0. *)
+(*     + simpl in H1. apply H1. *)
+(* Qed. *)
 
-(* A list has length > 0 iff there exists a head to the list.*)
-Theorem  length_hd_error : forall (A:Type) (l:list A), 1 <= length l <-> exists y:A, hd_error l = Some y.
-Proof.
-intros. split.
-- induction l.
-  + intros. inversion H.
-  + intros. exists a. reflexivity.
-- intros. destruct H. assert (x::(tl l) = l).
-  { symmetry. apply hd_error_tl_repr. split.
-    - apply H.
-    - reflexivity.
-  }
-  rewrite <- H0. simpl. induction (length (tl l)).
-  + reflexivity.
-  + apply le_S. apply IHn.
-Qed.
+(* (* A list has length > 0 iff there exists a head to the list.*) *)
+(* Theorem  length_hd_error : forall (A:Type) (l:list A), 1 <= length l <-> exists y:A, hd_error l = Some y. *)
+(* Proof. *)
+(* intros. split. *)
+(* - induction l. *)
+(*   + intros. inversion H. *)
+(*   + intros. exists a. reflexivity. *)
+(* - intros. destruct H. assert (x::(tl l) = l). *)
+(*   { symmetry. apply hd_error_tl_repr. split. *)
+(*     - apply H. *)
+(*     - reflexivity. *)
+(*   } *)
+(*   rewrite <- H0. simpl. induction (length (tl l)). *)
+(*   + reflexivity. *)
+(*   + apply le_S. apply IHn. *)
+(* Qed. *)
 
-(* The head of a list [b0++b1] is the head of list [b0] if [b0] is nonempty.*)
-Theorem hd_error_app : forall (b0 b1: list State) (a:State), hd_error b0 = Some a -> (hd_error (b0 ++ b1)) = Some a.
-  {
-    intros. induction b0.
-    - inversion H.
-    - simpl. simpl in H. apply H.
-  }
-Qed.
+(* (* The head of a list [b0++b1] is the head of list [b0] if [b0] is nonempty.*) *)
+(* Theorem hd_error_app : forall (b0 b1: list State) (a:State), hd_error b0 = Some a -> (hd_error (b0 ++ b1)) = Some a. *)
+(*   { *)
+(*     intros. induction b0. *)
+(*     - inversion H. *)
+(*     - simpl. simpl in H. apply H. *)
+(*   } *)
+(* Qed. *)
 
-(* If [computation_property] holds for [l0++l1] and [l0] is nonempty, [computation_property] holds for [l0]. *)
-Theorem computation_property_app :
-  forall (g:CGS) (q:State) (l0 l1: list State),
-    (1 <= (length l0)) -> computation_property g q (l0 ++ l1) -> computation_property g q l0.
-Proof.
-  intros. destruct H0. unfold computation_property. generalize dependent q. induction l0.
-  - intros. inversion H.
-  - intros. split.
-    + simpl in H0. simpl. apply H0.
-    + simpl. simpl in H1. simpl in H0. inversion H.
-      *
-        assert (hd_error l0 = None).
-        {
-          symmetry in H3. apply length_zero_iff_nil in H3.
-          rewrite H3. reflexivity.
-        }
-        rewrite H2. apply I.
-      * 
-        assert (length l0 > 0).
-        { unfold gt. unfold lt. apply H3. }
-        apply length_hd_error in H3. destruct H3. apply (hd_error_app l0 l1 x) in H3.
-        rewrite H3 in H1. destruct H1. apply (IHl0 H4 H5 x) in H3.
-        destruct H3.
-        rewrite H3. split.
-        -- apply H1.
-        -- apply H6.
-Qed.
+(* (* If [computation_property] holds for [l0++l1] and [l0] is nonempty, [computation_property] holds for [l0]. *) *)
+(* Theorem computation_property_app : *)
+(*   forall (g:CGS) (q:State) (l0 l1: list State), *)
+(*     (1 <= (length l0)) -> computation_property g q (l0 ++ l1) -> computation_property g q l0. *)
+(* Proof. *)
+(*   intros. destruct H0. unfold computation_property. generalize dependent q. induction l0. *)
+(*   - intros. inversion H. *)
+(*   - intros. split. *)
+(*     + simpl in H0. simpl. apply H0. *)
+(*     + simpl. simpl in H1. simpl in H0. inversion H. *)
+(*       * *)
+(*         assert (hd_error l0 = None). *)
+(*         { *)
+(*           symmetry in H3. apply length_zero_iff_nil in H3. *)
+(*           rewrite H3. reflexivity. *)
+(*         } *)
+(*         rewrite H2. apply I. *)
+(*       *  *)
+(*         assert (length l0 > 0). *)
+(*         { unfold gt. unfold lt. apply H3. } *)
+(*         apply length_hd_error in H3. destruct H3. apply (hd_error_app l0 l1 x) in H3. *)
+(*         rewrite H3 in H1. destruct H1. apply (IHl0 H4 H5 x) in H3. *)
+(*         destruct H3. *)
+(*         rewrite H3. split. *)
+(*         -- apply H1. *)
+(*         -- apply H6. *)
+(* Qed. *)
 
-(* The nonempty prefix of a [q]-computation is a [q]-computation. *)
-Theorem computation_property_prefix :
-  forall (g:CGS) (n:nat) (q:State) (l:computation g q),
-    computation_property g q (firstn (S n) (proj1_sig l)).
-Proof.
-  intros. destruct l. unfold proj1_sig. destruct c.
-  pose proof (hd_error_app (firstn (S n) x) (skipn (S n) x) q) as H1.
-  assert ((hd_error (firstn (S n) x)) = Some q).
-  {
-    simpl. destruct x.
-    - apply H.
-    - simpl. simpl in H. apply H.
-  }
-  apply H1 in H2.
-  destruct (length_hd_error State x).
-  assert (exists y, hd_error x = Some y).
-  { exists q. apply H. }
-  apply H4 in H5.
-  pose proof (@computation_property_app g q (firstn (S n) x) (skipn (S n) x)).
-  assert (1 <= length (firstn (S n) x)).
-  {
-    induction x.
-    - inversion H.
-    - simpl. induction (firstn n x).
-      + reflexivity.
-      + simpl. apply le_S. apply IHl.
-  }
-  assert (@computation_property g q x).
-  {
-    unfold computation_property. split.
-    - apply H.
-    - apply H0.
-  }
-  rewrite firstn_skipn in H6.
-  apply (H6 H7 H8).
-Qed.
+(* (* The nonempty prefix of a [q]-computation is a [q]-computation. *) *)
+(* Theorem computation_property_prefix : *)
+(*   forall (g:CGS) (n:nat) (q:State) (l:computation g q), *)
+(*     computation_property g q (firstn (S n) (proj1_sig l)). *)
+(* Proof. *)
+(*   intros. destruct l. unfold proj1_sig. destruct c. *)
+(*   pose proof (hd_error_app (firstn (S n) x) (skipn (S n) x) q) as H1. *)
+(*   assert ((hd_error (firstn (S n) x)) = Some q). *)
+(*   { *)
+(*     simpl. destruct x. *)
+(*     - apply H. *)
+(*     - simpl. simpl in H. apply H. *)
+(*   } *)
+(*   apply H1 in H2. *)
+(*   destruct (length_hd_error State x). *)
+(*   assert (exists y, hd_error x = Some y). *)
+(*   { exists q. apply H. } *)
+(*   apply H4 in H5. *)
+(*   pose proof (@computation_property_app g q (firstn (S n) x) (skipn (S n) x)). *)
+(*   assert (1 <= length (firstn (S n) x)). *)
+(*   { *)
+(*     induction x. *)
+(*     - inversion H. *)
+(*     - simpl. induction (firstn n x). *)
+(*       + reflexivity. *)
+(*       + simpl. apply le_S. apply IHl. *)
+(*   } *)
+(*   assert (@computation_property g q x). *)
+(*   { *)
+(*     unfold computation_property. split. *)
+(*     - apply H. *)
+(*     - apply H0. *)
+(*   } *)
+(*   rewrite firstn_skipn in H6. *)
+(*   apply (H6 H7 H8). *)
+(* Qed. *)
 
-(* A function generating the [n+1]-long prefix of a [q]-computation.*)
-Definition computation_prefix
-           (g:CGS)
-           (q:State)
-           (l: computation g q)
-           (n:nat)
-           : computation g q
-:=
-  @exist (list State)
-         (computation_property g q)(* (fun l => computation_property g q l) *)
-         (firstn (S n) (proj1_sig l))
-         (computation_property_prefix g n q l).
+(* (* A function generating the [n+1]-long prefix of a [q]-computation.*) *)
+(* Definition computation_prefix *)
+(*            (g:CGS) *)
+(*            (q:State) *)
+(*            (l: computation g q) *)
+(*            (n:nat) *)
+(*            : computation g q *)
+(* := *)
+(*   @exist (list State) *)
+(*          (computation_property g q)(* (fun l => computation_property g q l) *) *)
+(*          (firstn (S n) (proj1_sig l)) *)
+(*          (computation_property_prefix g n q l). *)
 
-Check computation_prefix.
+(* Check computation_prefix. *)
 
 
 (* There is always a move available called [nothing], which if performed by every player fails to change state. *)
-Parameter nothing: Move.
-Axiom nothing_always_enabled : forall (g:CGS) (q:State) (p:Player), g.(e) q p nothing = true.
-Axiom nothing_does_nothing : forall (g:CGS) (q:State), g.(d) q (fun _ => nothing) = q.
-
-
-(* A strategy is a function from computations to moves, representing what a player would do in a particular play-through. *)
-Definition strategy (g:CGS) (p:Player) : Set := forall (q:State) (l:computation g q), {m:Move | g.(e) q p m = true}.
-
-Definition strat_nothing (g: CGS) (p:Player) : strategy g p :=
-  fun q _ => exist (fun m => g.(e) q p m = true) nothing (nothing_always_enabled g q p).
 
 (* A coalition is a set of players. *)
 Definition coalition : Set := Player -> bool.
@@ -204,47 +197,104 @@ Definition coalition : Set := Player -> bool.
 (* Coalition complement. *)
 Definition coal_comp (c:coalition) : coalition := fun p:Player => negb (c p).
 
-(* Definition grand (g:CGS) : coalition := g.(lp). *)
-(* Definition nobody : coalition := nil. *)
-(* Definition coal_comp (g:CGS) (c:coalition) : coalition := *)
-(*   let x := fix fx (y z:coalition) *)
-(*              := match y with *)
-(*                 | nil => z *)
-(*                 | a::y' => if existsb (beq_player a) c then fx y' z else fx y' (a::z) *)
-(*                 end *)
-(*   in x g.(lp) nil. *)
+Definition grand (g:CGS) : coalition := fun _ => true.
+Definition nobody : coalition := fun _ => false.
 
-(* Definition coal_union (c1 c2 : coalition) : coalition := c1 ++ c2. *)
+Definition coal_union (c1 c2 : coalition) : coalition := fun p => orb (c1 p) (c2 p).
 
-(*
-Definition coal_intersection (c1 c2: coalition) : coalition :=
-  let x := fix fx (y1 y2 z: coalition)
-*)
+Definition coal_intersection (c1 c2: coalition) : coalition := fun p => andb (c1 p) (c2 p).
+
+
+Parameter nothing: Move.
+Axiom nothing_always_enabled : forall (g:CGS) (q:State) (p:Player), g.(e) q p nothing = true.
+Axiom nothing_does_nothing : forall (g:CGS) (q:State), g.(d) q (fun _ _ => nothing) = q.
+
+
+(* A strategy is a function from computations to moves, representing what a player would do in a particular play-through. *)
+
+(* Inductive strategy (g:CGS) (p:Player) : (nonempty State) -> Move -> Set := *)
+(*   strat : forall (l:nonempty State) (m:Move) *)
+(*                  (ENABLED: g.(e) (nonempty_last l) p m = true), *)
+(*     strategy g p l m. *)
+
+(* Definition strat_nothing (g:CGS) (p:Player) := *)
+(*   fun l => strat g p l nothing (nothing_always_enabled g (nonempty_last l) p). *)
+
+
+Definition strategy (g:CGS) (p:Player) : Set := forall (l:nonempty State) (q:State) (CPL: computation_property g q l), Move.
+
+Definition strategy_legal (g:CGS) (p:Player) (s:strategy g p) :=
+  forall (l:nonempty State) (q:State) (CPL: computation_property g q l),
+    g.(e) (nonempty_last l) p (s l q CPL) = true.
+
+Definition strat_nothing (g: CGS) (p:Player) : strategy g p :=
+  fun l _ _ => nothing.
+
+Check strat_nothing.
+
+Theorem nothing_always_legal : forall (g:CGS) (p:Player),
+    strategy_legal g p (strat_nothing g p).
+Proof.
+  unfold strategy_legal. intros. apply nothing_always_enabled.
+Qed.
 
 (* [strategy_set] is a type representing unique strategies only of members in the coalition. *)
-Definition strategy_set (g:CGS) (c:coalition) : Set := forall (p:Player), c p = true -> strategy g p.
+Inductive strategy_set (g:CGS) (c:coalition) : Set :=
+| strat_set : forall (p:Player)
+                     (COAL: c p = true)
+                     (s: strategy g p)
+                     (SL: strategy_legal g p s),
+    strategy_set g c.
+
+
+(* Strategy set where members of the coalition do nothing. *)
+Definition ss_nothing (g:CGS) (c:coalition) := fun p COAL => strat_set g c p COAL (strat_nothing g p) (nothing_always_legal g p).
+
+Check ss_nothing.
 
 (* Whether a particular move vector obeys a given strategy set. *)
-Definition strategy_set_enabled (g:CGS) (c:coalition) (ss:strategy_set g c) (q:State) (l:computation g q) (mv:move_vec q) :=
-  forall (p:Player) (H:c p = true),
-    mv p = proj1_sig (ss p H q l).
-  
-(* Strategy set where members of the coalition do nothing. *)
-Definition ss_nothing (g:CGS) (c:coalition) : strategy_set g c := fun p _ => strat_nothing g p.
+Definition strategy_set_enabled
+           (g:CGS)
+           (c:coalition)
+           (ss:strategy_set g c)
+           (l:nonempty State)
+           (q:State)
+           (CPL: computation_property g q l)
+           (mv:move_vec) :=
+  match ss with
+  | strat_set _ _ p _ s _ =>  mv (nonempty_last l) p  = s l q CPL
+  end.
+(* TODO make [strategy_set], [strategy] inductive *)
 
 
+Inductive outcomes (g:CGS) (c: coalition) : (strategy_set g c) -> nonempty State -> Prop :=
+| outcomes_two : forall (ss:strategy_set g c) (q1 q2:State)
+                        (m: move_vec)
+                        (CPL: computation_property g q1 (q1:::q2::nil))
+                        (ENABLED: strategy_set_enabled g c ss (q1:::q2::nil) q1 CPL m)
+                        (DELTA: g.(d) q1 m = q2),
+    outcomes g c ss (q1:::q2::nil)
+| outcomes_cons : forall (ss:strategy_set g c) (q:State)
+                         (l:nonempty State)
+                         (m:move_vec)
+                         (CPL: computation_property g q (nonempty_cons q l))
+                         (ENABLED : strategy_set_enabled g c ss (nonempty_cons q l) q CPL m)
+                         (OUT: outcomes g c ss l),
+      outcomes g c ss (nonempty_cons q l).
+           
+                        (* TODO finish redefining outcomes *)
 
 (* Property checking whether a given computation obeys a strategy set in all successive states. *)
-Definition outcomes (g:CGS) (q:State) (c:coalition) (ss:strategy_set g c) (l: computation g q) : Prop
-:=
-  forall (i:nat),
-    S i  < (length (proj1_sig l)) ->
-    forall (m:move_vec (nth i (proj1_sig l) q))
-           (p:Player)
-           (H: c p = true),
-    let x := computation_prefix g q l i in
-    m p = proj1_sig (ss p H q x) ->
-    g.(d) (nth i (proj1_sig l) q) m = (nth (S i) (proj1_sig l) q).
+(* Definition outcomes (g:CGS) (q:State) (c:coalition) (ss:strategy_set g q c) (l: list State) (CPL: computation_property g q l) : Prop *)
+(* := *)
+(*   forall (i:nat), *)
+(*     S i  < (length l) -> *)
+(*     forall (m:move_vec) *)
+(*            (p:Player) *)
+(*            (H: c p = true), *)
+(*     let x := firstn i l in *)
+(*     m (nth i l q) p = ss p H x CPL -> *)
+(*     g.(d) (nth i l q) m = (nth (S i) l q). *)
 
 
 
@@ -263,7 +313,7 @@ Inductive sentence : Set :=
 Notation "p //\\ q" := (land p q) (at level 30).
 Notation "p \\// q" := (lor p q) (at level 30).
 Notation "!! p" := (lnot p)  (at level 30).
-Notation "p --> q" := (lnot (land (lnot p) q)) (at level 30).
+Notation "p --> q" := (lor (lnot p) q) (at level 30).
 Notation "<< c >>o p" := (possible_next c p) (at level 50).
 Notation "<< c >>^ p" := (possible_once c  p) (at level 50).
 Notation "<< c >># p" := (possible_always c p) (at level 50).
@@ -275,8 +325,8 @@ Notation "[[ c ]] p %% q" := (lnot (possible_until c (lnot q) p)) (at level 50).
 
 Check forall  (g:CGS) (q:State) (c: coalition),
     exists (ss:strategy_set g c),
-      forall (l:computation g q),
-        outcomes g q c ss l.
+      forall (l:nonempty State),
+        outcomes g c ss l.
 
 (* Variable not_helper : CGS -> State -> sentence -> Prop. *)
 
@@ -284,7 +334,7 @@ Check forall  (g:CGS) (q:State) (c: coalition),
 (* | verifiesObs: forall (g: CGS) (q: State) (a: Observable), *)
 (*     g.(o) q = a -> verifiesI g q (obs a) *)
 (* | verifiesNot: forall (g: CGS) (q: State) (phi: sentence), *)
-(*     ~ not_helper g q phi -> *)
+(*     (verifiesI g q phi -> False) -> *)
 (*     verifiesI g q (!! phi) *)
 (* | verifiesAnd: forall (g: CGS) (q: State) (phi1 phi2: sentence), *)
 (*     verifiesI g q phi1 -> *)
@@ -312,44 +362,59 @@ Check forall  (g:CGS) (q:State) (c: coalition),
 
     
     
-Fixpoint verifies (g:CGS) (q:State) (phi:sentence) :Prop :=
+Fixpoint verifies (g:CGS) (q:State) (phi:sentence) : Prop :=
   match phi with
-  | obs a => g.(o) q = a
+  | obs a => beq_observable (g.(o) q) a = true
   | !! a => ~ (verifies g q a)
   | a //\\ b => (verifies g q a) /\ (verifies g q b)
   | a \\// b => (verifies g q a) \/ (verifies g q b)
   | <<c>>o a => exists (ss:strategy_set g c),
-                forall (l:computation g q),
-                  outcomes g q c ss l ->
-                  (verifies g (nth 1 (proj1_sig l) q) a)
+                forall (l:nonempty State) (CPL: computation_property g q l),
+                  outcomes g c ss l ->
+                  (verifies g (nonempty_nth 1 l q) a)
   | <<c>>^ a => exists (ss:strategy_set g c),
-                forall (l:computation g q),
-                  outcomes g q c ss l ->
+                forall (l:nonempty State) (CPL:computation_property g q l),
+                  outcomes g c ss l ->
                   exists (n:nat),
-                    (verifies g (nth n (proj1_sig l) q) a)
+                    (verifies g (nonempty_nth n l q) a)
   | <<c>># a => exists (ss:strategy_set g c),
-                forall (l:computation g q),
-                  outcomes g q c ss l ->
+                forall (l:nonempty State) (CPL:computation_property g q l),
+                  outcomes g c ss l ->
                   forall (n:nat),
-                    (verifies g (nth n (proj1_sig l) q) a)
+                    (verifies g (nonempty_nth n l q) a)
   | <<c>> a %% b => exists (ss:strategy_set g c),
-                    forall (l:computation g q),
-                      outcomes g q c ss l ->
+                forall (l:nonempty State) (CPL:computation_property g q l),
+                      outcomes g c ss l ->
                       exists (n:nat),
-                        ((verifies g (nth n (proj1_sig l) q) b)
+                        ((verifies g (nonempty_nth n l q) b)
                          /\ forall (m:nat),
-                            m < n -> (verifies g (nth m (proj1_sig l) q) a))
+                            m < n -> (verifies g (nonempty_nth m l q) a))
   end.
+(* TODO write tactic to step through the fixpoint.
 
+The way that I know how to do this is to write lemmas that show
+what happens on one step. Eg:
+Lemma verifies_step_and: verifies(g q (a//\\b)) = 
+     verifies g q a /\ verifies g q b.
+Proof.
+unfold _.
+simpl _.
+reflexivity.
+Qed.
+
+Ltac stepverifies := first [rewrite verifies_step_and, rewrite verifies_step_or, rewrite verifies_step_*];
+Ltac simplpverifies := repeat stepverifies.
+ *)
 Definition invariant (g1 g2:CGS) : Prop := forall (phi:sentence) (q:State),
     verifies g1 q phi <-> verifies g2 q phi.
     
 (* TODO: invariance. *)
 (* TODO: proof calculus *)
 
-Definition spec : Type := sentence -> Prop.
+Definition spec : Type := State -> sentence -> Prop.
 
-Definition g_in_spec (sp:spec) (g:CGS) (q:State) : Prop := forall (phi:sentence), sp phi -> verifies g q phi.
+Definition g_in_spec (sp:spec) (g:CGS) (q:State) : Prop := forall (phi:sentence), sp q phi -> verifies g q phi.
+
 
 Theorem coal_comp_comp : forall c, coal_comp (coal_comp c) = c.
 Proof.
@@ -376,83 +441,18 @@ Proof.
     }
     simpl. intros. apply H.
     destruct H0. exists x. intros. apply H0 in H1. destruct H1. exists x0.
-    apply H. apply H1.
+    apply H. apply H1. apply CPL.
   - simpl. intros. apply NNPP in H. destruct H. exists x. intros.
     apply H in H0. destruct H0. exists x0.
-    apply NNPP in H0. apply H0.
-    
+    apply NNPP in H0. apply H0. apply CPL.
 Qed.
 
 
 Theorem computation_property_q : forall (g:CGS) (q:State),
-    computation_property g q (q::nil).
+    computation_property g q (q:::nil).
 Proof.
-  unfold computation_property. split.
-  - reflexivity.
-  - unfold computation_property_fix. simpl. apply I.
-Qed.
-
-Definition computation_q (g:CGS) (q:State) : computation g q := @exist (list State) (computation_property g q) (q::nil) (computation_property_q g q).
-
-Theorem nth_computation_q : forall (g:CGS) (q:State) (n:nat),
-    let l := computation_q g q in
-    (nth n (proj1_sig l) q) = q.
-Proof.
-  intros. unfold computation_q in l. unfold l.
-    unfold proj1_sig. assert (forall n, length (q::nil) <= (S n)).
-    {
-      simpl. induction n0.
-      - reflexivity.
-      - apply le_S. apply  IHn0.
-    }
-    induction n.
-  - reflexivity.
-  - pose proof (H n). pose proof (nth_overflow _ q H0). apply H1.
-Qed.
-
-Theorem zeroth_computation_is_q : forall (g:CGS) (q:State) (l: computation g q),
-    (nth 0 (proj1_sig l) q) = q.
-Proof.
-  intros. destruct l. unfold computation_property in c. destruct c.
-  simpl. induction x.
-  - inversion e0.
-  - inversion e0. reflexivity.
-Qed.
-
-Axiom computation_eq : forall (g:CGS) (q:State) (l1 l2:computation g q),
-    l1 = l2 <-> (proj1_sig l1) = (proj1_sig l2).
-
-Theorem ith_succ : (forall (g:CGS) (q:State) (l:list State) (i:nat), computation_property g q l -> S i < length l -> succ g (nth i l q) (nth (S i) l q)).
-Proof.
-  intros. generalize dependent i. generalize dependent q.
-  induction l.
-  - intros. inversion H0.
-  - destruct l.
-    + intros. inversion H0. inversion H2.
-    + intros. inversion H. inversion H2.
-      assert (hd_error (s::l) = Some s).
-      {
-        reflexivity.
-      }
-      assert (computation_property g s (s::l)).
-      {
-        unfold computation_property. split.
-        - apply H5.
-        - apply H4.
-      }
-      pose proof (IHl s H6).
-      assert (forall (i:nat) (a b:State) (l:list State), nth i l b = nth (S i) (a::l) b).
-      {
-        intros. destruct l0.
-        - reflexivity.
-        - reflexivity.
-      }
-      rewrite (nth_indep _ _ s H0).
-      pose proof (Le.le_Sn_le _ _ H0). rewrite (nth_indep _ _ s H9).
-      induction i.
-      * simpl. apply H3.
-      * rewrite <- H8. rewrite <- H8. apply H7. simpl. simpl in H0.
-        apply le_S_n. apply H0.
+  intros.
+  apply computation_property_one.
 Qed.
 
 Theorem coalition_complement_next : forall (g:CGS) (q:State) (phi:sentence) (c:coalition),
@@ -469,3 +469,8 @@ Theorem coalition_complement_until : forall (g:CGS) (q:State) (phi psi:sentence)
     verifies g q (<<c>> phi %% psi) <-> verifies g q ([[coal_comp c]] phi %% psi).
 Proof.
 Admitted.
+
+(* Create HintDb verifies. *)
+(* Hint Resolve coalitiion_complement_next : verifies. *)
+
+(* auto with verifies *)
