NonEmpty.v
@@ -1,0 +1,37 @@
+Require Import List.
+
+Inductive nonempty (A:Type) : Type := mknonempty: A -> (list A) -> nonempty A.
+
+Notation "a ::: la" := (mknonempty _ a la) (at level 61).
+
+Definition ne : nonempty nat := 1 ::: nil.
+
+Definition nonempty_last {A:Type} (n:nonempty A) :=
+  match n with
+  | mknonempty _ a b => last b a
+  end.
+
+Definition nonempty_cons {A:Type} (a:A) (n:nonempty A) :=
+  match n with
+  | mknonempty _ b c => a:::b::c
+  end.
+
+Definition nonempty_head {A:Type} (n:nonempty A) :=
+  match n with
+  | mknonempty _ a b => a
+  end.
+
+Definition nonempty_nth {A:Type} (i:nat) (n:nonempty A) (d:A) :=
+  match i with
+  | 0 => match n with
+         | mknonempty _ a b => a
+         end
+  | S i' => match n with
+           | mknonempty _ a b => nth i' b d
+           end
+  end.
+
+Definition nonempty_length {A:Type} (n:nonempty A) :=
+  match n with
+  | mknonempty _ a b => S (length b)
+  end.
