VNM.v
@@ -12,10 +12,14 @@ Definition reachable_payoffs_property (g:CGS)
          (o:Observable)
   : Prop :=
   forall (p:Player),
-    c p ->
+    c p = true ->
     verifies g q (<< c >>^ (obs o)).
 
 Check reachable_payoffs_property.
+
+Definition reachable_payoffs (g:CGS) (q:State) (c:coalition) : Set
+  := {o:Observable | reachable_payoffs_property g q c o}.
+
 
 Definition spec_reachable_payoffs_property (sp:spec)
            (q:State)
@@ -25,23 +29,21 @@ Definition spec_reachable_payoffs_property (sp:spec)
     forall(g:CGS), g_in_spec sp g q ->
                              reachable_payoffs_property g q c o.
 
-Definition spec_reachable_payoffs (sp:spec) (q:State) (c:coalition) : Type
+Definition spec_reachable_payoffs (sp:spec) (q:State) (c:coalition) : Set
   := {o:Observable | spec_reachable_payoffs_property sp q c o}.
 
 Definition core (g:CGS) (q:State) (o: Observable)  : Prop :=
-  reachable_payoffs_property g q grand o
+  reachable_payoffs_property g q (grand g) o
   /\ (forall (o':Observable),
-         reachable_payoffs_property g q grand o' ->
+         reachable_payoffs_property g q (grand g) o' ->
          (forall (p:Player),
              assignment o' p <= assignment o p))
     /\ (forall c:coalition,
            (forall (o':Observable),
                reachable_payoffs_property g q c o' ->
                (forall (p:Player),
-                   c p ->
+                   c p = true ->
                    assignment o' p <= assignment o p))).
-
-Definition listp_to_coalition (lp:list Player) : coalition := fun p => In p lp.
 
 Axiom core_must_happen : forall (g:CGS) (q:State) (o:Observable),
     core g q o -> reachable_payoffs_property g q nobody o.
