test.v
@@ -6,7 +6,5 @@ Variable m:Move.
 
 Definition test_move_vec : move_vec q := fun p:Player => m.
 
-
-Definition test_move_function : move_function := fun (q:State) (p:Player) => m.
-
-  
+Check test_move_vec.  
+                         
